Language_Components/Imp_Ctl/Imp_Ctl.thy
@@ -45,7 +45,9 @@ definition imp_ctl_sem :: "syn' \<Rightarrow> 'x imp_state' \<Rightarrow> 'x imp
           | [cond, body] \<Rightarrow> cond# ((G z [body])#t)
           | _ \<Rightarrow> [] \<comment>\<open> error \<close>)
         | SwhileC \<Rightarrow>
-        (case l of [body] \<Rightarrow> (if (b \<noteq> 0) then body # (G z [body]) # t else t)
+        (case l of [body] \<Rightarrow> 
+          (if (b \<noteq> 0) then body # (G z [body]) # t 
+           else t)
          | _ \<Rightarrow> [] \<comment>\<open> error \<close>))
       , b))"
 text_raw \<open>%EndSnippet\<close>
@@ -68,11 +70,14 @@ definition imp_prio :: "(syn' \<Rightarrow> nat)" where
 text_raw \<open>%EndSnippet\<close>
 
 text_raw \<open>%Snippet gazelle__language_components__imp_ctl__imp_ctl__imp_sem_lifting_gen\<close>
-definition imp_sem_lifting_gen :: "(syn', 'x imp_state', 
-                                   ('x, _ ) state) lifting" where
+definition imp_sem_lifting_gen ::
+  "(syn', 'x imp_state', 
+   ('x, _ ) state) lifting" where
 "imp_sem_lifting_gen = 
- (schem_lift (SP NA NB)
-             (SP (SPRC imp_prio (SO NA)) (SP NX (SP (SPRI (SO NB)) NX))))"
+ (schem_lift
+    (SP NA NB)
+    (SP (SPRC imp_prio (SO NA))
+        (SP NX (SP (SPRI (SO NB)) NX))))"
 text_raw \<open>%EndSnippet\<close>
 
 definition imp_sem_l_gen :: "('s \<Rightarrow> syn') \<Rightarrow> 's \<Rightarrow> ('x, 'z :: Mergeableb) state \<Rightarrow> ('x, 'z) state" where
