Language_Components/Calc/Calc.thy
@@ -21,7 +21,8 @@ fun calc_sem :: "calc \<Rightarrow> calc_state \<Rightarrow> calc_state" where
   (x1, x2, x1 + x2)"
 | "calc_sem (Csub) (x1, x2, _) = (x1, x2, x1 - x2)"
 | "calc_sem (Cmul) (x1, x2, _) = (x1, x2, x1 * x2)"
-| "calc_sem (Cdiv) (x1, x2, _) = (x1, x2, divide_int_inst.divide_int x1 x2)"
+| "calc_sem (Cdiv) (x1, x2, _) = 
+  (x1, x2, divide_int_inst.divide_int x1 x2)"
 | "calc_sem (Cnum i) (x1, x2, _) = (x1, x2, i)"
 | "calc_sem (Cskip) st = st"
 text_raw \<open>%EndSnippet\<close>
