Paper_Examples/Lifting_Valid_Example.thy
@@ -4,12 +4,18 @@ begin
 
 text_raw \<open>%Snippet paper_examples__lifting_valid_example__lifting_valid_example\<close>
 lemma lifting_valid_example :
-  "lifting_valid (schem_lift (SP NC (SP NB NA)) 
-    (SP (SPRI (SO NA)) (SP (SPRC (\<lambda> _ . 1) (SO NB)) (SPRI (SO NC)))))
-(schem_lift_S (SP NC (SP NB NA)) 
-    (SP (SPRI (SO NA)) (SP (SPRC (\<lambda> _ . 1) (SO NB)) (SPRI (SO NC))))) "
+  "lifting_valid 
+  (schem_lift (SP NC (SP NB NA)) 
+    (SP (SPRI (SO NA)) 
+        (SP (SPRC (\<lambda> _ . 1) (SO NB)) 
+            (SPRI (SO NC)))))
+  (schem_lift_S (SP NC (SP NB NA)) 
+    (SP (SPRI (SO NA)) 
+        (SP (SPRC (\<lambda> _ . 1) (SO NB)) 
+        (SPRI (SO NC))))) "
   unfolding schem_lift_defs schem_lift_S_defs
-  by(fastforce intro: lifting_valid_standard lifting_ortho_standard )
+  by(fastforce intro: lifting_valid_standard 
+      lifting_ortho_standard )
 text_raw \<open>%EndSnippet\<close>
 
 end
