Paper_Examples/Prog1_Annotated.thy
@@ -29,78 +29,80 @@ definition prog1_annotated :: "int \<Rightarrow> int \<Rightarrow> syn gensyn" w
   , \<dagger> Sm (Sread (STR ''arg2'') (Reg_c))
     \<comment> \<open>reg c = i2; mem[''arg1''] = i1; mem[''arg2''] = i2; mem[''one''] = 1; mem[''acc''] = 0\<close>
   , \<dagger> Sb Sgtz
-    \<comment> \<open>reg c = i2; reg flag = (i2 @{verbatim >} 0) mem[''arg1''] = i1; mem[''arg2''] = i2; mem[''one''] = 1; mem[''acc''] = 0\<close>
+    \<comment> \<open>reg c = i2; reg flag = (i2 @{verbatim >} 0) mem[''arg1''] = i1; \<close>
+    \<comment> \<open>mem[''arg2''] = i2; mem[''one''] = 1; mem[''acc''] = 0\<close>
 
     \<comment> \<open>
-     LOOP INVARIANT I: exists idx such that:
-     reg flag = 1 iff idx @{verbatim >} 0;
-     mem[''arg1''] = i1; mem[''arg2''] = idx; mem[''one''] = 1;
-     mem[''acc''] = i1 * (i2 - idx);
-     i2 @{verbatim >=} idx;
-     
-     holds initially for idx = i2\<close>
+     LOOP INVARIANT I: exists idx such that: \<close>
+     \<comment> \<open> reg flag = 1 iff idx @{verbatim >} 0; \<close>
+     \<comment> \<open> mem[''arg1''] = i1; mem[''arg2''] = idx; mem[''one''] = 1; \<close>
+     \<comment> \<open> mem[''acc''] = i1 * (i2 - idx); \<close>
+     \<comment> \<open> i2 @{verbatim >=} idx; \<close>
+     \<comment> \<open>\<close>
+     \<comment> \<open> holds initially for idx = i2 \<close>
   , \<diamond> (Si SwhileC)
     [ \<comment> \<open>I; reg flag = 1\<close>
       \<diamond> (Ss Sseq)
-      [ \<comment> \<open>I; reg flag = 1. We can restate this as:
-            mem[''arg1''] = i1; mem[''arg2''] = idx; mem[''one''] = 1;
-            mem[''acc''] = i1 * (i2 - idx);
-            i2 @{verbatim >=} idx; idx @{verbatim >} 0\<close>
+      [ \<comment> \<open>I; reg flag = 1. \<close> 
+        \<comment> \<open> We can restate this as: \<close>
+        \<comment> \<open> mem[''arg1''] = i1; mem[''arg2''] = idx; mem[''one''] = 1; \<close>
+        \<comment> \<open> mem[''acc''] = i1 * (i2 - idx); \<close>
+        \<comment> \<open> i2 @{verbatim >=} idx; idx @{verbatim >} 0\<close>
         \<dagger> Sm (Sread (STR ''arg1'') (Reg_a))
-        \<comment> \<open>reg a = i1;
-            mem[''arg1''] = i1; mem[''arg2''] = idx; mem[''one''] = 1;
-     	      mem[''acc''] = i1 * (i2 - idx);
-     	      i2 @{verbatim >=} idx; idx @{verbatim >} 0\<close>
+        \<comment> \<open>reg a = i1; \<close>
+        \<comment> \<open> mem[''arg1''] = i1; mem[''arg2''] = idx; mem[''one''] = 1; \<close>
+        \<comment> \<open> mem[''acc''] = i1 * (i2 - idx); \<close>
+        \<comment> \<open> i2 @{verbatim >=} idx; idx @{verbatim >} 0\<close>
       , \<dagger> Sm (Sread (STR ''acc'') (Reg_b))
-        \<comment> \<open>reg a = i1; reg b = i1 * (i2 - idx);
-            mem[''arg1''] = i1; mem[''arg2''] = idx; mem[''one''] = 1;
-     	      mem[''acc''] = i1 * (i2 - idx);
-     	      i2 @{verbatim >=} idx; idx @{verbatim >} 0\<close>
+        \<comment> \<open>reg a = i1; reg b = i1 * (i2 - idx); \<close>
+        \<comment> \<open> mem[''arg1''] = i1; mem[''arg2''] = idx; mem[''one''] = 1; \<close>
+        \<comment> \<open> mem[''acc''] = i1 * (i2 - idx); \<close>
+        \<comment> \<open> i2 @{verbatim >=} idx; idx @{verbatim >} 0\<close>
       , \<dagger> Sc Cadd
-        \<comment> \<open>reg a = i1; reg b = i1 * (i2 - idx); reg c = i1 * (i2 - idx) + i1;
-            mem[''arg1''] = i1; mem[''arg2''] = idx; mem[''one''] = 1;
-     	      mem[''acc''] = i1 * (i2 - idx);
-     	      i2 @{verbatim >=} idx; idx @{verbatim >} 0\<close>
+        \<comment> \<open>reg a = i1; reg b = i1 * (i2 - idx); reg c = i1 * (i2 - idx) + i1; \<close>
+        \<comment> \<open> mem[''arg1''] = i1; mem[''arg2''] = idx; mem[''one''] = 1; \<close>
+        \<comment> \<open>mem[''acc''] = i1 * (i2 - idx); \<close>
+        \<comment> \<open> i2 @{verbatim >=} idx; idx @{verbatim >} 0\<close>
       , \<dagger> Sm (Swrite (STR ''acc'') (Reg_c))
-        \<comment> \<open>reg a = i1; reg b = i1 * (i2 - idx); reg c = i1 * (i2 - idx) + i1;
-            mem[''arg1''] = i1; mem[''arg2''] = idx; mem[''one''] = 1;
-     	      mem[''acc''] = i1 * (i2 - idx) + i1;
-     	      i2 @{verbatim >=} idx; idx @{verbatim >} 0\<close>
+        \<comment> \<open>reg a = i1; reg b = i1 * (i2 - idx); reg c = i1 * (i2 - idx) + i1; \<close>
+        \<comment> \<open> mem[''arg1''] = i1; mem[''arg2''] = idx; mem[''one''] = 1; \<close>
+        \<comment> \<open> mem[''acc''] = i1 * (i2 - idx) + i1; \<close>
+        \<comment> \<open> i2 @{verbatim >=} idx; idx @{verbatim >} 0\<close>
       , \<dagger> Sm (Sread (STR ''arg2'') (Reg_a))
-        \<comment> \<open>reg a = idx; reg b = i1 * (i2 - idx); reg c = i1 * (i2 - idx) + i1;
-            mem[''arg1''] = i1; mem[''arg2''] = idx; mem[''one''] = 1;
-     	      mem[''acc''] = i1 * (i2 - idx) + i1;
-     	      i2 @{verbatim >=} idx; idx @{verbatim >} 0\<close>
+        \<comment> \<open>reg a = idx; reg b = i1 * (i2 - idx); reg c = i1 * (i2 - idx) + i1; \<close>
+        \<comment> \<open>mem[''arg1''] = i1; mem[''arg2''] = idx; mem[''one''] = 1; \<close>
+        \<comment> \<open>mem[''acc''] = i1 * (i2 - idx) + i1; \<close>
+        \<comment> \<open>i2 @{verbatim >=} idx; idx @{verbatim >} 0\<close>
       , \<dagger> Sm (Sread (STR ''one'') (Reg_b))
-        \<comment> \<open>reg a = idx; reg b = 1; reg c = reg c = i1 * (i2 - idx) + i1;
-            mem[''arg1''] = i1; mem[''arg2''] = idx; mem[''one''] = 1;
-     	      mem[''acc''] = i1 * (i2 - idx) + i1;
-     	      i2 @{verbatim >=} idx; idx @{verbatim >} 0\<close>
+        \<comment> \<open>reg a = idx; reg b = 1; reg c = reg c = i1 * (i2 - idx) + i1; \<close>
+        \<comment> \<open>mem[''arg1''] = i1; mem[''arg2''] = idx; mem[''one''] = 1; \<close>
+        \<comment> \<open>mem[''acc''] = i1 * (i2 - idx) + i1; \<close>
+        \<comment> \<open>i2 @{verbatim >=} idx; idx @{verbatim >} 0\<close>
       , \<dagger> Sc Csub
-        \<comment> \<open>reg a = idx; reg b = 1; reg c = idx - 1;
-            mem[''arg1''] = i1; mem[''arg2''] = idx; mem[''one''] = 1;
-     	      mem[''acc''] = i1 * (i2 - idx) + i1;
-     	      i2 @{verbatim >=} idx; idx @{verbatim >} 0\<close>
+        \<comment> \<open>reg a = idx; reg b = 1; reg c = idx - 1; \<close>
+        \<comment> \<open>mem[''arg1''] = i1; mem[''arg2''] = idx; mem[''one''] = 1; \<close>
+        \<comment> \<open>mem[''acc''] = i1 * (i2 - idx) + i1; \<close>
+        \<comment> \<open>i2 @{verbatim >=} idx; idx @{verbatim >} 0\<close>
       , \<dagger> Sm (Swrite (STR ''arg2'') (Reg_c))
-        \<comment> \<open>reg a = idx; reg b = 1; reg c = idx - 1;
-            mem[''arg1''] = i1; mem[''arg2''] = idx - 1; mem[''one''] = 1;
-     	      mem[''acc''] = i1 * (i2 - idx) + i1;
-     	      i2 @{verbatim >=} idx; idx @{verbatim >} 0\<close>
+        \<comment> \<open>reg a = idx; reg b = 1; reg c = idx - 1; \<close>
+        \<comment> \<open>mem[''arg1''] = i1; mem[''arg2''] = idx - 1; mem[''one''] = 1; \<close>
+        \<comment> \<open>mem[''acc''] = i1 * (i2 - idx) + i1; \<close>
+        \<comment> \<open>i2 @{verbatim >=} idx; idx @{verbatim >} 0\<close>
       , \<dagger> Sm (Sread (STR ''arg2'') (Reg_c))
-        \<comment> \<open>reg a = idx; reg b = 1; reg c = idx - 1;
-            mem[''arg1''] = i1; mem[''arg2''] = idx - 1; mem[''one''] = 1;
-     	      mem[''acc''] = i1 * (i2 - idx) + i1;
-     	      i2 @{verbatim >=} idx; idx @{verbatim >} 0\<close>
+        \<comment> \<open>reg a = idx; reg b = 1; reg c = idx - 1;\<close>
+        \<comment> \<open>mem[''arg1''] = i1; mem[''arg2''] = idx - 1; mem[''one''] = 1;\<close>
+        \<comment> \<open>mem[''acc''] = i1 * (i2 - idx) + i1;\<close>
+        \<comment> \<open>i2 @{verbatim >=} idx; idx @{verbatim >} 0\<close>
       , \<dagger> Sb Sgtz
-        \<comment> \<open>reg a = idx; reg b = 1; reg c = idx - 1; reg flag = 1 iff idx' @{verbatim > } 0
-            mem[''arg1''] = i1; mem[''arg2''] = idx - 1; mem[''one''] = 1;
-     	      mem[''acc''] = i1 * (i2 - idx) + i1;
-     	      i2 @{verbatim >=} idx\<close>
-        \<comment> \<open>let idx' = idx - 1. Then:
-            reg flag = 1 iff idx' @{verbatim >} 0;
-            mem[''arg1''] = i1; mem[''arg2''] = idx'; mem[''one''] = 1;
-            mem[''acc''] = i1 * (i2 - (idx' + 1)) + i1 = i1 * (i2 - idx');
-            i2 @{verbatim >=} idx'\<close>
+        \<comment> \<open>reg a = idx; reg b = 1; reg c = idx - 1; reg flag = 1 iff idx' @{verbatim > } 0\<close>
+        \<comment> \<open>mem[''arg1''] = i1; mem[''arg2''] = idx - 1; mem[''one''] = 1;\<close>
+        \<comment> \<open>mem[''acc''] = i1 * (i2 - idx) + i1;\<close>
+        \<comment> \<open>i2 @{verbatim >=} idx\<close>
+        \<comment> \<open>let idx' = idx - 1. Then:\<close>
+        \<comment> \<open>reg flag = 1 iff idx' @{verbatim >} 0;\<close>
+        \<comment> \<open>mem[''arg1''] = i1; mem[''arg2''] = idx'; mem[''one''] = 1;\<close>
+        \<comment> \<open>mem[''acc''] = i1 * (i2 - (idx' + 1)) + i1 = i1 * (i2 - idx');\<close>
+        \<comment> \<open>i2 @{verbatim >=} idx'\<close>
         \<comment> \<open>Therefore invariant I is reestablished for idx'\<close>
       ]
     ]
